theories/Projection/ProjectionFun.v
@@ -59,32 +59,16 @@ destruct l=>//=.  apply/H.  eauto.
 simpl in *. rewrite negb_or in H2. ssa. 
 Qed. 
 
-(*Intermediate judgment that gives us induction principle to show Rolling_no_fv*)
-Inductive has_var (n : nat ) :  gType -> Prop := 
- | hv0  : has_var n (GVar n)
- | hv1 a u g0 : has_var n g0 -> has_var n (GMsg a u g0)
- | hv2 g gs a : In g gs -> has_var n g  -> has_var n (GBranch a gs)
- | hv3 g : has_var n (g [g GRec g .: GVar]) ->  has_var n (GRec g).
-Hint Constructors has_var. 
 
 
-
-Lemma has_var_subst : forall g n n' sigma, has_var n g -> has_var n' (sigma n)  ->  has_var n' g [g sigma]. 
-Proof. 
-move => g n n' sigma  H. elim : H n' sigma;rewrite //=;intros. 
-con. apply/H0. done. simpl. econstructor. apply/inP. apply/mapP. exists g0. apply/inP. done. eauto. 
-apply/H1. done. con. asimpl. move/H0 : H1. asimpl. done. 
-Qed. 
-
-
-Fixpoint econtractive2 g := 
+(*Fixpoint econtractive2 g := 
 match g with
 | EVar j => true
 | EEnd => true
 | EMsg _ _ _ g0 => econtractive2 g0
 | EBranch _ _ gs => all econtractive2 gs
 | ERec g0 => (eguarded 0 g0) && (econtractive2 g0)
-end. 
+end. *)
 
 Lemma project_econtractive2 : forall p g, econtractive2 (trans p g). 
 Proof. 
@@ -109,152 +93,7 @@ ssa. destruct n. simpl. exfalso. apply/negP. apply/H0. done.
 simpl. done. 
 Qed.
 
-Fixpoint gType_fv2 e :=
-  match e with
-  | GVar j => [:: j]
-  | GEnd => nil
-  | GMsg _ _ g0 => gType_fv2 g0
-  | GBranch _ gs => flatten (map gType_fv2 gs)
-  | GRec g0 => map predn (filter (fun n => n != 0) (gType_fv2 g0))
-  end.
 
-Definition gclosed g := forall n, n \notin gType_fv2 g.
-
-Lemma gType_fv2_ren : forall g sigma, (gType_fv2 g ⟨g sigma⟩) = map sigma (gType_fv2 g). 
-Proof. 
-elim;rewrite //=;intros. 
-rewrite -!map_comp. rewrite H.
-rewrite filter_map /=. clear H. asimpl. 
-elim : (gType_fv2 g). done. ssa. 
-destruct (eqVneq a 0). subst. simpl. ssa. 
-simpl. destruct a. done. simpl. f_equal. done. 
-rewrite -!map_comp. rewrite map_flatten. rewrite -!map_comp. 
-f_equal. apply/eq_in_map=> x xIn. simpl. auto. 
-Qed.
-
-Lemma gType_fv2_subst : forall g sigma, (gType_fv2 g [g sigma]) = flatten (map (sigma >> gType_fv2) (gType_fv2 g)). 
-Proof. 
-elim;rewrite //=;intros. 
-rewrite cats0. asimpl. done. 
-rewrite H. rewrite -!map_comp. 
-asimpl. rewrite filter_flatten.
-rewrite -!map_comp. rewrite !map_flatten.
-rewrite -map_comp.
-rewrite /comp. asimpl. clear H.
-elim : ( gType_fv2 g);try done. ssa. 
-destruct (eqVneq a 0). simpl. subst. simpl. done. 
-simpl. destruct a. done. simpl.
-f_equal. asimpl. rewrite gType_fv2_ren. 
-rewrite filter_map /=. rewrite -map_comp.
-clear i.  clear H. 
-elim : ( gType_fv2 (sigma a));try done. ssa. 
-f_equal. done. done.  
-
-rewrite -map_comp. 
-rewrite !map_flatten.  rewrite -!map_comp. 
-rewrite /comp. asimpl. 
-elim : l H. done. ssa. simpl.
-rewrite flatten_cat. f_equal. auto. apply/H. auto. 
-Qed.
-
-
-Lemma has_varP : forall g n, n \in gType_fv2 g -> has_var n g. 
-Proof. 
-elim=>//=;intros;auto. rewrite inE in H. rewrite (eqP H). done. 
-con. move : H0. move/mapP=>[]. intros. subst. rewrite mem_filter in p. ssa. 
-destruct x;try done. simpl. 
-move/H : H1. intros. apply/has_var_subst. eauto. simpl. con. 
-move/flattenP : H0=>[] x. move/mapP=>[]. intros. subst. econstructor. 
-apply/inP. eauto. eauto. 
-Qed.
-
-(*Cool Trick, when going from coinductive to negation of some structurally recursive boolean,
- intermediate step is to show boolean implies inductive unfolding judgment,
- it's negation is introduced into the context and the proof can be by induction on that.
- The technique informally says from the coinductive Rolling judgment and a proof
- that we will observe a variable in finite time, we can reach a contradiction,
- so there can be no free variables.
-*)
-Lemma Rolling_no_fv : forall g, Rolling g -> (forall n, n \notin gType_fv2 g).
-Proof. 
-intros. apply/negP. move/has_varP=>HH. elim : HH H;intros. 
-punfold H. inv H. inv H0. punfold H1. punfold H2. 
-punfold H1. inv H1. rewrite full_unf_subst in H2. apply/H0. 
-pfold. con. done. 
-Qed.
-
-
-Fixpoint endpoint_fv2 e :=
-  match e with
-  | EVar j => [:: j]
-  | EEnd => nil
-  | EMsg _ _ _ g0 => endpoint_fv2 g0
-  | EBranch _ _ gs => flatten (map endpoint_fv2 gs)
-  | ERec g0 => map predn (filter (fun n => n != 0) (endpoint_fv2 g0))
-  end.
-
-Definition eclosed e := forall n, n \notin endpoint_fv2 e.
-
-Lemma endpoint_fv2_ren : forall g sigma, (endpoint_fv2 g ⟨e sigma⟩) = map sigma (endpoint_fv2 g). 
-Proof. 
-elim;rewrite //=;intros. 
-rewrite -!map_comp. rewrite H.
-rewrite filter_map /=. clear H. asimpl. 
-elim : (endpoint_fv2 e). done. ssa. 
-destruct (eqVneq a 0). subst. simpl. ssa. 
-simpl. destruct a. done. simpl. f_equal. done. 
-rewrite -!map_comp. rewrite map_flatten. rewrite -!map_comp. 
-f_equal. apply/eq_in_map=> x xIn. simpl. auto. 
-Qed.
-
-Lemma endpoint_fv2_subst : forall g sigma, (endpoint_fv2 g [e sigma]) = flatten (map (sigma >> endpoint_fv2) (endpoint_fv2 g)). 
-Proof. 
-elim;rewrite //=;intros. 
-rewrite cats0. asimpl. done. 
-rewrite H. rewrite -!map_comp. 
-asimpl. Search _ ((filter _ (flatten _))). rewrite filter_flatten.
-rewrite -!map_comp. rewrite !map_flatten.
-rewrite -map_comp.
-rewrite /comp. asimpl. clear H.
-elim : ( endpoint_fv2 e);try done. ssa. 
-destruct (eqVneq a 0). simpl. subst. simpl. done. 
-simpl. destruct a. done. simpl.
-f_equal. asimpl. rewrite endpoint_fv2_ren. 
-rewrite filter_map /=. rewrite -map_comp.
-clear i.  clear H. 
-elim : ( endpoint_fv2 (sigma a));try done. ssa. 
-f_equal. done. done.  
-
-rewrite -map_comp. 
-rewrite !map_flatten.  rewrite -!map_comp. 
-rewrite /comp. asimpl. 
-elim : l H. done. ssa. simpl.
-rewrite flatten_cat. f_equal. auto. apply/H. auto. 
-Qed.
-
-
-
-
-Lemma endpoint_fv2_eunf : forall g n, (n \in endpoint_fv2 g) = (n \in endpoint_fv2 (eunf g)).  
-Proof. 
-case=>//=. intros. rewrite endpoint_fv2_subst. 
-apply/eq_iff. split. move/mapP=>[] x /=. rewrite mem_filter. ssa. subst. 
-apply/flattenP. destruct x;try done. simpl. 
-have : ((ERec e .: EVar) >> endpoint_fv2) = 
-([seq i.-1 | i <- endpoint_fv2 e & i != 0] .: fun n => [::n]).
-asimpl. simpl. f_equal. move=>->.
-exists ([::x]). 
-apply/mapP. exists x.+1. ssa. simpl. done. done. 
-move/flattenP=>[] x. move/mapP=>[] x0. intros. subst. destruct x0;try done.  
-move : q0. asimpl. simpl. rewrite inE. move/eqP. intros. subst. apply/mapP. exists x0.+1=>//=. 
-rewrite mem_filter. ssa. 
-Qed.
-
-Lemma endpoint_fv2_full_eunf : forall g n, (n \in endpoint_fv2 g) = (n \in endpoint_fv2 (full_eunf g)).  
-Proof. 
-intros. rewrite /full_eunf. remember (emu_height g). clear Heqn0. elim : n0 g. done. 
-intros. rewrite iterS. rewrite H. apply/endpoint_fv2_eunf. 
-Qed.
 
 
 
@@ -320,24 +159,8 @@ rewrite -!map_comp. destruct l. done. simpl. rewrite H. auto. done. done.
 Qed. 
 
 
-Lemma eguarded_sig2 : forall g sigma sigma' i, eguarded i g [e sigma] -> (forall n, eguarded i (sigma n) -> eguarded i (sigma' n)) -> eguarded i g [e sigma'].
-Proof.
-elim;rewrite /=;intros;try done.
-apply H0. done.
-asimpl. apply : H. eauto. move => n.  asimpl. simpl. intros. destruct n. done. simpl in *.
-move : H. rewrite /funcomp. specialize H1 with n. move : H0. asimpl.
-intros. rewrite -eguarded_ren_iff. move : H. rewrite -eguarded_ren_iff.  move/H1. done. 
-done. done. 
-Qed.
 
 
-Lemma  eguarded_fv : forall g v, v \notin endpoint_fv2 g -> eguarded v g.
-Proof.
-elim;rewrite /=;try done;intros.
-rewrite !inE in H. lia.
-apply H. move : H0. intros. apply/negP=>HH'. apply/negP. apply H0. apply/mapP. exists v.+1. rewrite mem_filter. ssa. done. 
-Qed.
- 
 Lemma project_subst  : forall p g sigma, trans p g [g sigma ] = (trans p g) [e sigma >> trans p ]. 
 Proof. 
 move => p. elim;intros;asimpl.  
@@ -486,122 +309,8 @@ Qed.
 
 
 
-Lemma CProj_Unravel : forall p g gc ec, Unravelg2 g gc ->  CProject gc p ec -> paco2 EQ_gen bot2 ec (etocoind (trans p g)). 
-Proof. 
-move => p. pcofix CIH. 
-intros. apply part_of_or_end in H1 as H1'. destruct H1'.
-move/ICpart_of_all2_iff : H=>g0.  
-have : part_of_all2 p g. apply/g0. done. 
-clear g0=>HH. 
-elim/part_of_all2_ind2 : HH gc ec H1 H0;intros. 
-- rewrite etocoind_full_eunf. rewrite proj_eq_full H0 /=.  destruct (comp_dir p a) eqn:Heqn;try done. cbn. 
-  punfold H2. inv H2. rewrite H0 in H3. inv H3. punfold H1. inv H1;try comp_disc;pc. 
-  rewrite Heqn in H9. inv H9. pfold. seq. con=>//=. eauto. 
-  have : ~ comp_dir p a by eauto. comp_disc. 
-
-- rewrite etocoind_full_eunf. rewrite proj_eq_full H2 /=.  destruct (comp_dir p a) eqn:Heqn;try done.
-  punfold H4. inv H4. rewrite H2 in H5. inv H5;pc. punfold H3. inv H3;pc;try comp_disc. 
-  rewrite -etocoind_full_eunf.   apply/H1; eauto. 
-  rewrite -etocoind_full_eunf.   apply/H1; eauto. pfold. con;eauto. 
-
-- rewrite etocoind_full_eunf. rewrite proj_eq_full H0 /=.  destruct (comp_dir p a) eqn:Heqn;try done. cbn. 
-  punfold H2. inv H2. rewrite H0 in H3. inv H3. punfold H1. inv H1;try comp_disc;pc. injt. 
-  rewrite Heqn in H7. inv H7. pfold. seq. con.  
-  rewrite -map_comp. clear H3 H2 H1  H7 H0. apply/Forall_ForallC. rewrite size_map//=. lia. 
-  move/ForallP : H11. elim : gs ecs es H6 H9 H8. case=>//=. case=>//=.
-  move => a0 l IH.   case=>//=. move => a1 l0 [] //=. move => a2 l1 [] Heq [] Heq2. intros. 
-  inv H8. inv H11. pclearbot. simpl in *. con;eauto. 
-  have : ~ comp_dir p a by eauto. comp_disc. 
-
-- rewrite etocoind_full_eunf. rewrite proj_eq_full H2 /=.  destruct (comp_dir p a) eqn:Heqn;try done.
-  punfold H4. inv H4. rewrite H2 in H5. inv H5;pc. punfold H3. inv H3;pc;try comp_disc. injt.
-  destruct gs;try done. destruct ecs;try done. simpl. 
-  rewrite -etocoind_full_eunf. destruct ecs;try done. inv H10.  pclearbot. simpl in *. 
-  apply/H1. simpl. eauto. apply/H0.  simpl. eauto. 2 : eauto. 
-  have : g2 = g2 \/ In g2 ecs. eauto. move/H13. ssa. pclearbot. done. 
-
-  destruct gs;try done. destruct ecs;try done. simpl. seq. pfold. con.
-  rewrite -etocoind_full_eunf. simpl.
-  inv H10. destruct ecs;try done. destruct H11;try done. destruct ecs;try done.  simpl in *. inv H9.  
-  simpl in *.
-  apply/H1. simpl. eauto. apply/H0.  simpl. eauto. 2 : eauto. pfold. con. 
-  move => HH. apply H6. econstructor 4.  2 : eauto. con.  done. 
-  punfold H7. inv H7. injt. inv H14. pclearbot. done.  
-
--  subst.  apply CProject_not_part in H1. have : ECEnd = etocoind EEnd. seq. done. 
-  move=>->. apply/paco2_mon. apply/EQ2_EQ. apply/project_project. pfold. con. con.
-  rewrite -part_of2_iff. 
-  rewrite ICpart_of_iff. eauto. eauto. 
-  rewrite -Rolling_iff. 
-  apply/Unravel_Rolling.  eauto. done.
-Qed.
 
 
-
-
-Lemma inotin : forall g i sigma, (forall n, i !=  sigma n) -> i \notin endpoint_fv2 g ⟨e sigma ⟩.
-Proof.
-elim;rewrite /=;try done;intros. rewrite !inE. specialize H with n. lia.
-apply/negP. move/mapP. case. ssa. subst. rewrite mem_filter in p. ssa. 
-destruct x;try done. ssa. apply/negP. apply/H. 2 : eauto. asimpl. intros.
-destruct n. done. ssa. asimpl. move: (H0 n).  lia. 
-apply/negP. move/flattenP. case. move=> x. rewrite -map_comp. move/mapP.  case. intros. subst. 
-apply/negP. apply/H. eauto. eauto. done. 
-Qed.
-
-Lemma econtractive2_ren : forall g sigma, injective sigma -> (forall n, n <= sigma n) ->  econtractive2  g -> econtractive2 g ⟨e sigma ⟩.
-Proof.
-elim;intros;simpl;try done. 
-asimpl. split_and. have : 0 = ( 0 .: sigma >> succn) 0. done. intros. rewrite {1}x.
-apply eguarded_ren. auto. ssa. apply/H=>//=. auto. intros. destruct n. simpl. done. ssa. asimpl. move : (H1 n). lia. ssa. ssa. 
-rewrite all_map. apply/allP. intro. intros. simpl. apply H. done.  done. done.  simpl in H2. apply (allP H2). done.
-Qed.
-
-
-Lemma econtractive2_subst : forall g sigma,econtractive2 g -> (forall n, econtractive2 (sigma n)) -> econtractive2 g [e sigma].
-Proof. 
-elim;rewrite /=;intros;try done. 
-asimpl. split_and. 
-apply/eguarded_sig2.
-instantiate (1 := (EVar 0 .: EVar  >>  ⟨e ↑ ⟩)).  asimpl. done.
-case. done. simpl. intros. apply/eguarded_fv. asimpl. apply/inotin. done.
-apply H. done.  intros. destruct n.  done. simpl. asimpl.  apply/econtractive2_ren. done. done. done.
-apply H. done.  intros. done. 
-rewrite all_map. apply/allP. intro. intros. simpl. apply H. done. apply (allP H0). done. done.
-Qed.
-
-
-
-
-
-(*Lemma emu_height_subst : forall g0 sigma, (forall n, 0 < emu_height (sigma n) -> eguarded n g0) -> econtractive2 g0 -> emu_height (g0[e sigma]) = emu_height g0.
-Proof. 
-elim; try solve [by rewrite /=];intros.
-asimpl. move : (H n). destruct (emu_height (sigma n)) eqn:Heqn. done. have : 0 < n0.+1 by lia. move => + HH. move/HH=>//=. lia. 
-simpl. f_equal. asimpl. apply H. case. rewrite //=. move=> n/=. move => HH. apply/H0. move : HH. asimpl. rewrite emu_height_ren //=. ssa. 
-Qed.*)
-
-
-
-
-
-
-
-
-Lemma econtractive_unf : forall g , econtractive2 g -> econtractive2 (eunf g). 
-Proof.
-intros. rewrite /eunf. destruct g;try done. apply/econtractive2_subst. ssa. case;done. 
-Qed.
-
-Lemma econtractive_iter_unf : forall k g , econtractive2 g -> econtractive2 (iter k eunf g). 
-Proof.
-elim;try done. intros. simpl. apply/econtractive_unf. ssa. 
-Qed.
-
-Lemma econtractive_full_eunf : forall g , econtractive2 g -> econtractive2 (full_eunf g). 
-Proof. 
-intros. rewrite /full_eunf. apply/econtractive_iter_unf. done. 
-Qed.
 
 Lemma emu_height_subst_contractive : forall g0 sigma, (forall n, 0 < emu_height (sigma n) -> eguarded n g0) -> econtractive2 g0 -> emu_height (g0[e sigma]) = emu_height g0.
 Proof. 
@@ -655,20 +364,63 @@ exfalso. apply/Heq. done.
 Qed.
 
 (*Lemma 11 in the paper*)
-Locate Unravele.
-Print Unravele. 
-Lemma Unraveling_of_trans : forall g p, gclosed g ->  paco2 (UnfUnravele \o Unravele2_gen) bot2 (trans p g) (etocoind (trans p g)).
+Lemma Unraveling_of_trans : forall g p, gclosed g ->  Unravele2 (trans p g) (etocoind (trans p g)).
 Proof. 
 intros. apply/Rolling_Unravele. apply/to_Rollinge. intros. apply/fv_proj_not=>//=.
 apply/project_econtractive2.
 Qed.
 
-(*Lemma Rolling_proj : forall p g, Rolling g -> Rollinge (trans p g). 
+
+
+Lemma trans_as_projection : forall p g gc ec, Unravelg2 g gc ->  CProject gc p ec -> paco2 EQ_gen bot2 ec (etocoind (trans p g)). 
 Proof. 
-intros. apply/to_Rollinge. intros. apply/negP. move/fv_proj=>HH. 
-move/Rolling_no_fv : H. move/(_ n). rewrite HH //=.   
-apply/project_econtractive2. 
-Qed.*)
+move => p. pcofix CIH. 
+intros. apply part_of_or_end in H1 as H1'. destruct H1'.
+move/ICpart_of_all2_iff : H=>g0.  
+have : part_of_all2 p g. apply/g0. done. 
+clear g0=>HH. 
+elim/part_of_all2_ind2 : HH gc ec H1 H0;intros. 
+- rewrite etocoind_full_eunf. rewrite proj_eq_full H0 /=.  destruct (comp_dir p a) eqn:Heqn;try done. cbn. 
+  punfold H2. inv H2. rewrite H0 in H3. inv H3. punfold H1. inv H1;try comp_disc;pc. 
+  rewrite Heqn in H9. inv H9. pfold. seq. con=>//=. eauto. 
+  have : ~ comp_dir p a by eauto. comp_disc. 
+
+- rewrite etocoind_full_eunf. rewrite proj_eq_full H2 /=.  destruct (comp_dir p a) eqn:Heqn;try done.
+  punfold H4. inv H4. rewrite H2 in H5. inv H5;pc. punfold H3. inv H3;pc;try comp_disc. 
+  rewrite -etocoind_full_eunf.   apply/H1; eauto. 
+  rewrite -etocoind_full_eunf.   apply/H1; eauto. pfold. con;eauto. 
+
+- rewrite etocoind_full_eunf. rewrite proj_eq_full H0 /=.  destruct (comp_dir p a) eqn:Heqn;try done. cbn. 
+  punfold H2. inv H2. rewrite H0 in H3. inv H3. punfold H1. inv H1;try comp_disc;pc. injt. 
+  rewrite Heqn in H7. inv H7. pfold. seq. con.  
+  rewrite -map_comp. clear H3 H2 H1  H7 H0. apply/Forall_ForallC. rewrite size_map//=. lia. 
+  move/ForallP : H11. elim : gs ecs es H6 H9 H8. case=>//=. case=>//=.
+  move => a0 l IH.   case=>//=. move => a1 l0 [] //=. move => a2 l1 [] Heq [] Heq2. intros. 
+  inv H8. inv H11. pclearbot. simpl in *. con;eauto. 
+  have : ~ comp_dir p a by eauto. comp_disc. 
+
+- rewrite etocoind_full_eunf. rewrite proj_eq_full H2 /=.  destruct (comp_dir p a) eqn:Heqn;try done.
+  punfold H4. inv H4. rewrite H2 in H5. inv H5;pc. punfold H3. inv H3;pc;try comp_disc. injt.
+  destruct gs;try done. destruct ecs;try done. simpl. 
+  rewrite -etocoind_full_eunf. destruct ecs;try done. inv H10.  pclearbot. simpl in *. 
+  apply/H1. simpl. eauto. apply/H0.  simpl. eauto. 2 : eauto. 
+  have : g2 = g2 \/ In g2 ecs. eauto. move/H13. ssa. pclearbot. done. 
+
+  destruct gs;try done. destruct ecs;try done. simpl. seq. pfold. con.
+  rewrite -etocoind_full_eunf. simpl.
+  inv H10. destruct ecs;try done. destruct H11;try done. destruct ecs;try done.  simpl in *. inv H9.  
+  simpl in *.
+  apply/H1. simpl. eauto. apply/H0.  simpl. eauto. 2 : eauto. pfold. con. 
+  move => HH. apply H6. econstructor 4.  2 : eauto. con.  done. 
+  punfold H7. inv H7. injt. inv H14. pclearbot. done.  
+
+-  subst.  apply CProject_not_part in H1. have : ECEnd = etocoind EEnd. seq. done. 
+  move=>->. apply/paco2_mon. apply/EQ2_EQ. apply/project_project. pfold. con. con.
+  rewrite -part_of2_iff. 
+  rewrite ICpart_of_iff. eauto. eauto. 
+  rewrite -Rolling_iff. 
+  apply/Unravel_Rolling.  eauto. done.
+Qed.
 
 Lemma CProject_EQ : forall p g e0 e1, CProject g p e0 -> paco2 EQ_gen bot2 e0 e1 -> CProject g p e1. 
 Proof. 
@@ -711,20 +463,23 @@ Proof.
 intros. exists (trans p g). ssa. 
 apply/Unravele_iff.
 suff : exists ec', (trans p g) << Unravele_gen >> ec'. case. 
-intros. have :  paco2 EQ_gen bot2 ec (etocoind (trans p g)). apply/CProj_Unravel. eauto. done. 
+intros. have :  paco2 EQ_gen bot2 ec (etocoind (trans p g)). apply/trans_as_projection. eauto. done. 
 intros. apply/Unravele_iff.  apply/Unravele_eq. apply/EQ_sym. eauto.  
-apply/Rolling_Unravele. 
-apply/Rolling_proj. apply/Unravel_Rolling. eauto.
+apply/Rolling_Unravele. apply/to_Rollinge. intros. apply/fv_proj_not. 
+apply/Rolling_no_fv. apply/Unravel_Rolling. eauto. apply project_econtractive2.
 exists (etocoind (trans p g)).
-apply/Unravele_iff. apply/Rolling_Unravele. apply/Rolling_proj. 
-apply Unravel_Rolling in H0. done. 
+apply/Unravele_iff. apply/Rolling_Unravele. 
+apply/to_Rollinge. intros. apply/fv_proj_not. 
+apply/Rolling_no_fv. apply/Unravel_Rolling. eauto. apply project_econtractive2.
+(*apply Unravel_Rolling in H0. *)
 rewrite /project. case_if. done. 
 exfalso. have : ~  projectb g p (trans p g) .  destruct ( projectb g p (trans p g) );try done. 
 intros. apply / x. clear H1. 
 apply/projectb_iff.
-apply/ICProject_iff. exists gc. exists (etocoind (trans p g)). ssa.
-apply/Rolling_Unravele. apply/Rolling_proj. apply/Unravel_Rolling. eauto.
-apply/CProject_EQ. eauto. apply/CProj_Unravel. eauto. done.
+apply/ICProject_iff. exists gc. exists (etocoind (trans p g)).
+ssa. apply/Rolling_Unravele/to_Rollinge. intros. apply/fv_proj_not. 
+apply/Rolling_no_fv. apply/Unravel_Rolling. eauto. apply project_econtractive2.
+apply/CProject_EQ. eauto. apply/trans_as_projection. eauto. done.
 Qed.
 
 
