README.md
@@ -1,4 +1,9 @@
-This repository is the Coq mechanisation that accompanies the paper "Sound and Complete Projection of Multi Party Session Types"
+This repository is the Coq mechanisation that accompanies the paper "Sound and Complete Projection of Multi Party Session Types". 
+We now describe the conceptual mapping from the paper to the code 
+
+Section 2 (Global Types, Local Types, and Standard Projection):
+Global and Local type syntax: theories/Syntax.v
+
 
 Notes:
 Difference Unravele (paper and main theorem) and Unravele2 (used internally)
@@ -6,3 +11,4 @@ to_coseq trick (Finite, why we need it)
 
 Lemma 27, should have ( (has_tree g) && (pair_next_rec p nil (project_predP p) true (g,e))) on the right hand side
 
+Unravelg <-> Unravelg2
